First result on scopability

Reachability.v
@@ -1,11 +1,12 @@
 From Celsius Require Export Trees.
 From Celsius Require Export Eval.
-Require Import ssreflect ssrbool. 
+Require Import ssreflect ssrbool.
 
 Require Import List.
 Import ListNotations.
 Open Scope nat_scope.
 Open Scope list_scope.
+Require Import Sets.Ensembles.
 
 Module Reachability.
   Import Eval.Evaluator.
@@ -14,31 +15,40 @@ Module Reachability.
   Inductive reachability : Store -> Loc -> Loc ->Prop :=
   |rch_heap  : forall l σ,  l < (dom σ) -> (reachability σ l l)
   |rch_trans : forall l0 l1 l2 C ω σ, (reachability σ l0 l1) -> (getObj σ l1 = Some (C, ω)) -> (exists f, (getVal ω f = Some l2)) -> (l2 < dom σ) -> (reachability σ l0 l2).
-
   Notation "σ ⊨ l1 ⇝ l2" := (reachability σ l1 l2) (at level 80, l1 at level 99).
+
+  Definition LocSet := (Ensemble Loc).
+  Notation "l ∈ L" := (In Loc L l) (at level 80).
+  Notation "L ⊆ L'" := (Included Loc L L') (at level 80).
+
+
+  Definition reachability_set σ (L: LocSet) l := exists l', (l' ∈ L) /\ (σ ⊨ l' ⇝ l).
+  Notation "σ ⊫ L ⇝ l" := (reachability_set σ L l) (at level 80, l at level 99, L at level 99).
 
 
   Definition reachable_cold (σ: Store) (l: Loc) := (l < dom σ).
   Notation "σ ⊨ l : 'cold'" := (reachable_cold σ l) (at level 80, l at level 99).
-  
+   Notation "σ ⊫ L : 'cold'" := (forall l, (l ∈ L) -> reachable_cold σ l) (at level 80, L at level 99).
+
   Definition reachable_warm (σ: Store) (l: Loc) := (exists C ω args fields methods , (getObj σ l) = Some (C, ω) /\ ((ct C) = Some (class args fields methods)) /\ (length fields <= length ω)).
   Notation "σ ⊨ l : 'warm'" := (reachable_warm σ l) (at level 80, l at level 99).
-  
-  Definition reachable_hot  (σ: Store) (l: Loc) :=(forall (l': Loc), σ ⊨ l ⇝ l' -> (σ ⊨ l' : cold)).  
-  Notation "σ ⊨ l : 'hot'"  := (reachable_hot σ l) (at level 80, l at level 99).
+  Notation "σ ⊫ L : 'warm'" := (forall l, (l ∈ L) -> reachable_warm σ l) (at level 80, L at level 99).
 
-  
-  
+  Definition reachable_hot  (σ: Store) (l: Loc) :=(forall (l': Loc), σ ⊨ l ⇝ l' -> (σ ⊨ l' : cold)).
+  Notation "σ ⊨ l : 'hot'"  := (reachable_hot σ l) (at level 80, l at level 99).
+  Notation "σ ⊫ L : 'hot'" := (forall l, (l ∈ L) -> reachable_hot σ l) (at level 80, L at level 99).
+
   Lemma reachability_trans: (forall σ l1 l2 l3, (σ ⊨ l1 ⇝ l2) -> (σ ⊨ l2 ⇝ l3) -> (σ ⊨ l1 ⇝ l3)).
   Proof.
     intros σ l1 l2 l3 H1 H2.
-    induction H2 => //. 
-    apply (rch_trans l1 l2 l3 C ω σ (IHreachability H1) H H0 H3). 
+    induction H2 => //.
+    apply (rch_trans l1 l2 l3 C ω σ (IHreachability H1) H H0 H3).
   Qed.
   Lemma reachability_hot: forall (σ: Store) (l l': Loc), σ ⊨ l: hot -> σ ⊨ l ⇝ l' -> σ ⊨ l': hot.
   Proof.
     intros σ l l' H1 H2 l'' H3.
     apply (H1 l'' ((reachability_trans _ _ _ _) H2 H3)).
-  Qed. 
-  
-End Reachability.              
+  Qed.
+
+
+End Reachability.
