Scopability.v
@@ -1,0 +1,42 @@
+From Celsius Require Export Trees.
+From Celsius Require Export Eval.
+From Celsius Require Export PartialMonotonicity.
+From Celsius Require Export Reachability.
+From Celsius Require Export Compatibility.
+Require Import ssreflect ssrbool.
+
+Require Import List.
+Import ListNotations.
+Open Scope nat_scope.
+Require Import Sets.Ensembles.
+
+
+Module Scopability.
+  Import Eval.Evaluator.
+  Import Reachability.Reachability.
+
+  Definition scoping (σ1 σ2: Store) (L1 L2: Ensemble Loc) := forall l, l < (dom σ1) -> (σ2 ⊫ L2 ⇝ l) -> σ1 ⊫ L1 ⇝ l.
+  Notation "a ⋖ b" := (scoping (fst b) (fst a) (snd b) (snd a)) (at level 80).
+
+  Definition scoping_preservation (σ1 σ2: Store) L :=
+    forall σ0 (L0 L1: Ensemble Loc),
+      (forall l, (l ∈ L0) -> l < (dom σ0)) ->
+      (forall l, (l ∈ L1) -> l < (dom σ1)) ->
+      (σ1, L)  ⋖ (σ0, L0) ->
+      (σ1, L1) ⋖ (σ0, L0) ->
+      (σ2, L1) ⋖ (σ0, L0).
+
+  Notation "σ1 ⇝ σ2 ⋖ L" := (scoping_preservation σ1 σ2 L) (at level 80, L at level 99, σ2 at level 99).
+
+  (* Results : *)
+
+  Lemma scoping_reflexivity : forall (σ: Store) (L1 L2: Ensemble Loc), (Included Loc L1 L2) -> ((σ, L1) ⋖ (σ, L2)).
+  Proof.
+    unfold scoping, reachability_set.
+    simpl.
+    intros.
+    move: H1 => [l' [Hl'1 Hl'2]].
+    exists l'; split => //.
+    unfold Included in H.
+    auto.
+  Qed.
